WIP (does not compile yet)

src/axiomatic/sim.v
@@ -29,6 +29,15 @@ Remove Hints plus_n_O.
 
 Hint Resolve gstep_coh gstep_inc coh_wf.
 
+Lemma foo (P Q : Prop) : P -> (P -> Q) -> P /\ Q.
+Proof. tauto. Qed.
+
+Lemma helper P (a: event) :
+  forall x, (fun x => P x \/ (eq a x)) x <-> P x \/ a = x.
+Proof.
+eauto.
+Qed.
+
 Section Monotone.
 
 Definition monotone (mo : event -> event -> Prop) f :=
@@ -88,9 +97,9 @@ Variable sc : event -> event -> Prop.
 
 Definition sim_msg (m: Message.t) b:=
   << VAL: Some m.(Message.val) = (val b) >> /\
-  << UR: forall l, max_value f (fun a => msg_rel urr acts sb rmw rf sc l a b) ((m.(Message.released)).(Capability.ur) l) >> /\
-  << RW: forall l, max_value f (fun a => msg_rel rwr acts sb rmw rf sc l a b) ((m.(Message.released)).(Capability.rw) l) >> /\
-  << SC: forall l, max_value f (fun a => msg_rel scr acts sb rmw rf sc l a b) ((m.(Message.released)).(Capability.sc) l) >>.
+  << UR: forall l, max_value f (fun a => msg_rel urr acts sb rmw rf sc l a b) (LocFun.find l (m.(Message.released)).(Capability.ur)) >> /\
+  << RW: forall l, max_value f (fun a => msg_rel rwr acts sb rmw rf sc l a b) (LocFun.find l (m.(Message.released)).(Capability.rw)) >> /\
+  << SC: forall l, max_value f (fun a => msg_rel scr acts sb rmw rf sc l a b) (LocFun.find l (m.(Message.released)).(Capability.sc)) >>.
 
 Definition sim_cell_helper b from msg :=
   << SIMMSG: sim_msg msg b >> /\ 
@@ -107,44 +116,52 @@ Definition sim_mem (mem: Memory.t) :=
   forall l, sim_cell (mem l) l.
 
 Definition sim_rel rel i :=
-  << REL_UR: forall l' l, max_value f (t_rel urr acts sb rmw rf sc i l' l) ((rel l').(Capability.ur) l) >> /\
-  << REL_RW: forall l' l, max_value f (t_rel rwr acts sb rmw rf sc i l' l) ((rel l').(Capability.rw) l) >> /\
-  << REL_SC: forall l' l, max_value f (t_rel scr acts sb rmw rf sc i l' l) ((rel l').(Capability.sc) l) >>.
+  << REL_UR: forall l' l, max_value f (t_rel urr acts sb rmw rf sc i l' l) 
+    (LocFun.find l (LocFun.find l' rel).(Capability.ur)) >> /\
+  << REL_UR: forall l' l, max_value f (t_rel rwr acts sb rmw rf sc i l' l) 
+    (LocFun.find l (LocFun.find l' rel).(Capability.rw)) >> /\
+  << REL_UR: forall l' l, max_value f (t_rel scr acts sb rmw rf sc i l' l) 
+    (LocFun.find l (LocFun.find l' rel).(Capability.sc)) >>.
 
 Definition sim_cur cur i :=
-  << CUR_UR: forall l, max_value f (t_cur urr acts sb rmw rf sc i l) (cur.(Capability.ur) l) >> /\
-  << CUR_RW: forall l, max_value f (t_cur rwr acts sb rmw rf sc i l) (cur.(Capability.rw) l) >> /\
-  << CUR_SC: forall l, max_value f (t_cur scr acts sb rmw rf sc i l) (cur.(Capability.sc) l) >>.
+  << CUR_UR: forall l, max_value f (t_cur urr acts sb rmw rf sc i l) 
+    (LocFun.find l cur.(Capability.ur)) >> /\
+  << CUR_RW: forall l, max_value f (t_cur rwr acts sb rmw rf sc i l) 
+    (LocFun.find l cur.(Capability.rw)) >> /\
+  << CUR_SC: forall l, max_value f (t_cur scr acts sb rmw rf sc i l) 
+    (LocFun.find l cur.(Capability.sc)) >>.
 
 Definition sim_acq acq i :=
-  << ACQ_UR: forall l, max_value f (t_acq urr acts sb rmw rf sc i l) (acq.(Capability.ur) l) >> /\
-  << ACQ_RW: forall l, max_value f (t_acq rwr acts sb rmw rf sc i l) (acq.(Capability.rw) l) >> /\
-  << ACQ_SC: forall l, max_value f (t_acq scr acts sb rmw rf sc i l) (acq.(Capability.sc) l) >>.
+  << ACQ_UR: forall l, max_value f (t_acq urr acts sb rmw rf sc i l) 
+    (LocFun.find l acq.(Capability.ur)) >> /\
+  << ACQ_RW: forall l, max_value f (t_acq rwr acts sb rmw rf sc i l) 
+    (LocFun.find l acq.(Capability.rw)) >> /\
+  << ACQ_SC: forall l, max_value f (t_acq scr acts sb rmw rf sc i l) 
+    (LocFun.find l acq.(Capability.sc)) >>.
 
 Definition sim_commit commit i :=
   << CUR: sim_cur commit.(Commit.cur) i >> /\
   << ACQ: sim_acq commit.(Commit.acq) i >> /\
   << REL: sim_rel commit.(Commit.rel) i >>.
 
-Definition sim_local local i :=
-  sim_commit local.(Local.commit) i.
-
 End Simulation.
-
-Definition sim_f f (op_st: Configuration.t) (ax_st: Machine.configuration) :=
-  << LOCAL: forall i foo local (TID: IdentMap.find i (Configuration.threads op_st) = Some (foo, local)),
-                sim_local f (acts ax_st) (sb ax_st) (rmw ax_st) (rf ax_st) (sc ax_st) local i >> /\
-  << SC: forall l, max_value f (S_tm (acts ax_st) (sb ax_st) (rmw ax_st) (rf ax_st) l) (Configuration.sc op_st l)  >> /\
-  << MEM: sim_mem f (acts ax_st) (sb ax_st) (rmw ax_st) (rf ax_st) (sc ax_st) op_st.(Configuration.memory) >>.
 
 Definition sim (op_st: Configuration.t) (ax_st: Machine.configuration) :=
   << COH: Coherent (acts ax_st) (sb ax_st) (rmw ax_st) (rf ax_st) (mo ax_st) (sc ax_st) >> /\
   << WF_OP_ST: Configuration.wf op_st >> /\
   << CONS_OP_ST: Configuration.consistent op_st >> /\
-  << NO_PROMISES: forall i foo local (TID: IdentMap.find i (Configuration.threads op_st) = Some (foo, local)),
+  << NO_PROMISES: forall i foo local 
+        (TID: IdentMap.find i (Configuration.threads op_st) = Some (foo, local)),
          local.(Local.promises) = Memory.bot>> /\
   << STATES: ts ax_st = IdentMap.map fst (Configuration.threads op_st) >> /\
-  << TIME: exists f, << MONOTONE: monotone (mo ax_st) f >> /\  << SIM: sim_f f op_st ax_st >>>>.
+  << TIME: exists f, 
+    << MONOTONE: monotone (mo ax_st) f >> /\  
+    << SIM_COMMIT: forall i foo local
+        (TID: IdentMap.find i (Configuration.threads op_st) = Some (foo, local)),
+        sim_commit f (acts ax_st) (sb ax_st) (rmw ax_st) (rf ax_st) (sc ax_st) local.(Local.commit) i >> /\
+    << SIM_SC_MAP: forall l, max_value f (S_tm (acts ax_st) (sb ax_st) (rmw ax_st) (rf ax_st) l) 
+         (LocFun.find l (Configuration.sc op_st))>> /\
+    << SIM_MEM: sim_mem f (acts ax_st) (sb ax_st) (rmw ax_st) (rf ax_st) (sc ax_st) (Configuration.memory op_st)  >> >>.
 
 Lemma find_mapD A B tid (f: A -> B) x y :
   IdentMap.find tid (IdentMap.map f x) = Some y ->
@@ -179,7 +196,7 @@ Qed.
 
 (* Next two lemmas from old Vbase:
  *)
-Lemma fun_if 
+(* Lemma fun_if 
 (A B : Type) (f : A -> B) (b : bool) (vT vF : A)
 : f (if b then vT else vF) = if b then f vT else f vF.
 Proof. by case b. Qed.
@@ -193,11 +210,25 @@ Proof. by case b. Qed.
 Lemma if_same 
 (A : Type) (b : bool): forall f : A,
   (if b then f else f) = f.
-Proof. desf. Qed.
+Proof. desf. Qed. *)
 
 Lemma tm_join a b l :
   TimeMap.join a b l =  Time.join (a l) (b l).
 Proof.  ins. Qed.
+
+Lemma tm_find_join l a b :
+  LocFun.find l (TimeMap.join a b) = 
+  Time.join (LocFun.find l a) (LocFun.find l b).
+Proof.
+Admitted.
+
+Lemma tm_find_singleton l l' t  :
+  LocFun.find l (TimeMap.singleton l' t) = 
+    if (Loc.eq_dec l l') then t else Time.bot.
+Proof.
+desf.
+Qed.
+
 
 Lemma tm_singleton l t  :
   TimeMap.singleton l t l = t.
@@ -238,6 +269,16 @@ apply TimeMap.bot_spec.
 apply TimeMap.join_l.
 Qed.
 
+Lemma cap_join_bot a  :
+  Capability.join a Capability.bot =  a.
+Proof.
+eapply Capability.antisym.
+apply Capability.join_spec.
+apply Capability.le_PreOrder.
+apply Capability.bot_spec.
+apply Capability.join_l.
+Qed.
+
 Lemma max_value_singleton f b t (T: t = f b):
   max_value f (eq b) t.
 Proof.
@@ -246,18 +287,102 @@ by apply Time.le_lteq; eauto.
 exists b; splits; try apply Time.le_lteq; eauto.
 Qed.
 
-Lemma max_value_same_set f f' P P' t :
-  max_value f P t ->
-  (forall x, P x <-> P' x) ->  
-  (forall x, P x -> f' x = f x) ->  
-  max_value f' P' t.
+Lemma max_value_new_f f f' P t 
+  (MAX: max_value f P t) (F: forall x, P x -> f' x = f x):
+  max_value f' P t.
 Proof.
-  unfold max_value; ins; desf; splits; ins.
-  rewrite H1; specialize (H0 a); desf; eauto.
-  exists a_max; rewrite H1; specialize (H0 a_max); desf; split; auto.
+unfold max_value in *; ins; desf; splits; ins.
+rewrite F; auto.
+exists a_max; rewrite F; auto.
 Qed.
 
+Lemma max_value_same_set f P P' t 
+  (MAX: max_value f P t) (SAME: forall x, P' x <-> P x):   
+  max_value f P' t.
+Proof.
+  unfold max_value in *; ins; desf; splits; ins.
+  specialize (SAME a); desf; eauto.
+  exists a_max; specialize (SAME a_max); desf; split; auto.
+Qed.
 
+Lemma max_value_join f P P' P'' t t'
+  (MAX: max_value f P t) (MAX':  max_value f P' t')
+  (SAME: forall x, P'' x <-> P x \/ P' x):
+  max_value f P'' (Time.join t t').
+Proof.
+unfold max_value in *; ins; desf; splits; ins.
+apply SAME in INa1; desf.
+all: try by etransitivity; eauto; eauto using Time.join_l, Time.join_r. 
+destruct (Time.le_lt_dec (f a_max) (f a_max0)); [exists a_max0|exists a_max]; splits.
+all: try rewrite SAME; eauto.
+all: try (apply Time.join_spec; eauto;
+       etransitivity; eauto; rewrite Time.le_lteq; eauto). 
+Qed.
+
+Lemma max_value_loc f f' P P' t b
+  (MAX: max_value f P t)
+  (SAME: forall x, P' x <-> P x \/ x = b)
+  (F: forall x, P x -> f' x = f x):
+  max_value f' P'  (Time.join t (f' b)).
+Proof.
+eapply max_value_join with (P':= eq b); eauto.
+eapply max_value_new_f with (f:=f); eauto.
+eapply max_value_singleton; done.
+ins; specialize (SAME x); desf; split; ins.
+apply SAME in H; desf; eauto.
+apply SAME0; desf; eauto.
+Qed.
+(* 
+Lemma max_value_join_loc f f' P P' P'' t t' b
+  (MAX: max_value f P t) (MAX':  max_value f P' t')
+  (SAME: forall x, P'' x <-> P x \/ P' x \/ x = b)
+  (F: forall x, P x \/ P' x -> f' x = f x):
+  max_value f' P'' (Time.join (Time.join (f' b) t) t').
+Proof.
+eapply max_value_join with (P:= fun x => P x \/ x = b); eauto.
+rewrite Time.join_comm.
+eapply max_value_loc; eauto.
+eapply max_value_new_f with (f:=f); eauto.
+ins; specialize (SAME x).
+tauto.
+Qed.
+
+Lemma max_value_join_loc' f f' P P' P'' t t' b
+  (MAX: max_value f P t) (MAX':  max_value f P' t')
+  (SAME: forall x, P'' x <-> P x \/ P' x \/ x = b)
+  (F: forall x, P x \/ P' x -> f' x = f x):
+  max_value f' P'' (Time.join (Time.join t (f' b)) t').
+Proof.
+rewrite (Time.join_comm t).
+eapply max_value_join_loc; eauto.
+Qed.
+
+Lemma max_value_join_loc'' f f' P P' P'' t t' b
+  (MAX: max_value f P t) (MAX':  max_value f P' t')
+  (SAME: forall x, P'' x <-> P x \/ P' x \/ x = b)
+  (F: forall x, P x \/ P' x -> f' x = f x):
+  max_value f' P'' (Time.join t' (Time.join t (f' b))).
+Proof.
+rewrite Time.join_comm.
+eapply max_value_join_loc'; eauto.
+Qed.
+
+Lemma max_value_join_join_loc f f' P P' P'' P''' t t' t'' b
+  (MAX: max_value f P t) (MAX':  max_value f P' t') (MAX'':  max_value f P'' t'')
+  (SAME: forall x, P''' x <-> P x \/ P' x \/ P'' x \/ x = b)
+  (F: forall x, P x \/ P' x \/ P'' x -> f' x = f x):
+max_value f' P''
+  (Time.join t (Time.join (Time.join t' (f' b)) t'')).
+Admitted.
+
+Lemma max_value_join_loc1 f f' P P' P'' t t' l b (LOC: loc b = Some l):
+  max_value f P t ->
+  max_value f P' t' ->
+  (forall x, P'' x <-> P x \/ P' x \/ x = b /\ loc x = Some l) ->
+  (forall x, P x \/ P' x -> f' x = f x) ->  
+  max_value f' P'' (Time.join t (Time.join t' (f' b))).
+Proof.
+Admitted.
 
 Lemma max_value_join_if f f' P P' P'' t t' (cond : bool):
   max_value f P t ->
@@ -283,14 +408,8 @@ unfold max_value; ins; desf; splits; ins.
   apply Time.join_spec; eauto using Time.bot_spec.
 Qed.
 
-Lemma max_value_join f f' P P' P'' t t':
-  max_value f P t ->
-  max_value f P' t' ->
-  (forall x, P'' x <-> P x \/ P' x) ->
-  (forall x, P'' x -> f' x = f x) ->  
-  max_value f' P'' (Time.join t t').
-Proof.
-Admitted.
+
+
 
 Lemma max_value_join_if2 f f' P P' P'' t t' (pred:Prop) (cond : {pred} + {~pred}):
   max_value f P t ->
@@ -315,7 +434,7 @@ unfold max_value; ins; desf; splits; ins.
   rewrite H2; rewrite H1; splits; eauto.
   apply Time.join_spec; eauto using Time.bot_spec.
 Qed.
-
+ *)
 
 (* Lemma my_Time_join_l a b c:
 Time.le a b ->
@@ -342,6 +461,7 @@ Qed. *)
   (Time.join (Capability.ur (Commit.cur (Local.commit local)) l')
      (if LocSet.Facts.eq_dec l l' then f' a else Time.bot))
  *)
+(*
 Lemma max_value_join_loc f f' P P' t l l' b (LOC: loc b = Some l):
   max_value f P t ->
   (forall x, P' x <-> P x \/ x = b /\ loc x = Some l') ->
@@ -371,7 +491,8 @@ Lemma max_value_join_if_loc f f' P P' P'' t t' (cond : bool) l l' b (LOC: loc b 
      (if cond then t' else Time.bot)).
 Proof.
 ins.
-eapply max_value_join_if with (f:=f') (P:= fun x=>P x \/ b = x /\ l = l') (P':=P'); 
+
+
 try edone.
 - eapply max_value_join_if2 with (f:=f'); eauto.
 eapply max_value_same_set; eauto.
@@ -381,36 +502,35 @@ apply max_value_singleton; eauto.
 split; ins; desf; eauto.
 apply H1 in H4; desf; eauto.
 Qed.
-
-Lemma sim_local_other_threads acts sb rmw rf mo sc acts' sb' rmw' rf' mo' sc'
-  a (GSTEP: gstep acts sb rmw rf mo sc acts' sb' rmw' rf' mo' sc' a)
-  (COH: Coherent acts sb rmw rf mo sc) 
-  f i (NEQ: i <> thread a) local (LOCAL: sim_local f acts sb rmw rf sc local i):
-    sim_local f acts' sb' rmw' rf' sc' local i.
+ *)
+Lemma sim_commit_other_threads_silent acts sb rmw rf mo sc
+  (COH: Coherent acts sb rmw rf mo sc) f f' i commit
+  (LOCAL: sim_commit f acts sb rmw rf sc commit i)
+  (F: forall a, (In a acts) -> f' a = f a) :
+    sim_commit f' acts sb rmw rf sc commit i.
 Proof.
-unfold sim_local, sim_commit, sim_cur, sim_acq, sim_rel in *; desf; splits;
-ins; eapply max_value_same_set; try edone; intro; symmetry.
-all: try eapply gstep_t_cur_other;  
-     try eapply gstep_t_acq_other;  
-     try eapply gstep_t_rel_other;  
-     eauto 2 using gstep_urr_a, gstep_rwr_a, gstep_scr_a, urr_mon, rwr_mon, scr_mon.
+unfold sim_commit, sim_cur, sim_acq, sim_rel in *; desf; splits; ins.
+all: eapply max_value_new_f; eauto.
+all: ins; apply F; eauto with acts.
 Qed.
 
-Lemma sim_local_other_threads' acts sb rmw rf mo sc acts' sb' rmw' rf' mo' sc'
+Lemma sim_commit_other_threads acts sb rmw rf mo sc acts' sb' rmw' rf' mo' sc'
   a (GSTEP: gstep acts sb rmw rf mo sc acts' sb' rmw' rf' mo' sc' a)
   (COH: Coherent acts sb rmw rf mo sc) 
-  f f' i (NEQ: i <> thread a) local 
-  (LOCAL: sim_local f acts sb rmw rf sc local i)
+  f f' i (NEQ: i <> thread a) commit 
+  (LOCAL: sim_commit f acts sb rmw rf sc commit i)
   (F: forall a, (In a acts) -> f' a = f a) :
-    sim_local f' acts' sb' rmw' rf' sc' local i.
+    sim_commit f' acts' sb' rmw' rf' sc' commit i.
 Proof.
-unfold sim_local, sim_commit, sim_cur, sim_acq, sim_rel in *; desf; splits;
-ins; eapply max_value_same_set; try edone; intro; symmetry.
-all: try eapply gstep_t_cur_other;  
+unfold sim_commit, sim_cur, sim_acq, sim_rel in *; desf; splits; ins.
+all: eapply max_value_same_set.
+all: try match goal with
+       | [|- max_value _ _ _] => eapply max_value_new_f with (f:=f); eauto with acts
+     end.
+all: ins; try eapply gstep_t_cur_other;  
      try eapply gstep_t_acq_other;  
      try eapply gstep_t_rel_other;  
      eauto 2 using gstep_urr_a, gstep_rwr_a, gstep_scr_a, urr_mon, rwr_mon, scr_mon.
-all: symmetry; apply F; eauto with acts.
 Qed.
 
 Lemma gstep_tm_to_a acts sb rmw rf mo sc acts' sb' rmw' rf' mo' sc'
@@ -492,12 +612,12 @@ eapply monotone_converse with (acts:=(a :: acts)); eauto.
 - rewrite gstep_non_write_mo with (mo':=mo'); eauto.
   rewrite <- ACT_STEP.
   cdes COH0; cdes WF; eauto.
-- intro. red in INa. red in INa.
-  unfold seq, eqv_rel in INa; desc; subst.
+- intro.
   eapply Coherent_scr_rel; eauto.
   eapply gstep_non_write_mo with (mo:=mo); eauto.
-  eapply scr_rel_mon; eauto.
-  eexists; eauto.
+  eapply gstep_scr_rel_nonwrite with (acts:=acts); eauto.
+  unfold scr_rel, msg_rel, m_rel, seq, eqv_rel in *; desc; subst.
+  eauto.
 Qed.
 
 Lemma Readable_full acts sb rmw rf mo sc acts' sb' rmw' rf' mo' sc'
@@ -527,6 +647,161 @@ constructor; try intro.
   ins; eapply Coherent_scr with (mo:=mo');  eauto with acts.
   eapply scr_actb; eauto.
 - eapply Readable_msg_sc; eauto with acts.
+Qed.
+
+Lemma commit_step_read
+ acts sb rmw rf mo sc op_st
+(COH : Coherent acts sb rmw rf mo sc)
+(f : event -> Time.t)
+(MONOTONE : monotone mo f)
+(SIM_SC_MAP : forall l : Loc.t,
+             max_value f (S_tm acts sb rmw rf l) (LocFun.find l (Configuration.sc op_st)))
+(l : Loc.t)
+(v : Const.t)
+(b : event)
+(from : Time.t)
+(rel : Capability.t)
+(VAL : Some (Message.val {| Message.val := v; Message.released := rel |}) = val b)
+(UR : forall l : Loc.t,
+     max_value f (fun a : event => msg_rel urr acts sb rmw rf sc l a b)
+       (LocFun.find l
+          (Capability.ur
+             (Message.released {| Message.val := v; Message.released := rel |}))))
+(RW : forall l : Loc.t,
+     max_value f (fun a : event => msg_rel rwr acts sb rmw rf sc l a b)
+       (LocFun.find l
+          (Capability.rw
+             (Message.released {| Message.val := v; Message.released := rel |}))))
+(SC : forall l : Loc.t,
+     max_value f (fun a : event => msg_rel scr acts sb rmw rf sc l a b)
+       (LocFun.find l
+          (Capability.sc
+             (Message.released {| Message.val := v; Message.released := rel |}))))
+(FROM : Time.lt from (f b))
+(FROMRMW : forall a : event, (rf;; rmw) a b -> from = f a)
+(acts0 : list event)
+(sb0 rmw0 rf0 mo0 sc0 : event -> event -> Prop)
+(lang : Language.t)
+(st st' : Language.state lang)
+(commit : Commit.t)
+(a : event)
+(o : Ordering.t)
+(LABa : lab a = Aload l v o)
+(GSTEP : gstep acts sb rmw rf mo sc acts0 sb0 rmw0 rf0 mo0 sc0 a)
+(CUR_UR : forall l : Loc.t,
+         max_value f (t_cur urr acts sb rmw rf sc (thread a) l)
+           (LocFun.find l (Capability.ur (Commit.cur commit))))
+(CUR_RW : forall l : Loc.t,
+         max_value f (t_cur rwr acts sb rmw rf sc (thread a) l)
+           (LocFun.find l (Capability.rw (Commit.cur commit))))
+(CUR_SC : forall l : Loc.t,
+         max_value f (t_cur scr acts sb rmw rf sc (thread a) l)
+           (LocFun.find l (Capability.sc (Commit.cur commit))))
+(ACQ_UR : forall l : Loc.t,
+         max_value f (t_acq urr acts sb rmw rf sc (thread a) l)
+           (LocFun.find l (Capability.ur (Commit.acq commit))))
+(ACQ_RW : forall l : Loc.t,
+         max_value f (t_acq rwr acts sb rmw rf sc (thread a) l)
+           (LocFun.find l (Capability.rw (Commit.acq commit))))
+(ACQ_SC : forall l : Loc.t,
+         max_value f (t_acq scr acts sb rmw rf sc (thread a) l)
+           (LocFun.find l (Capability.sc (Commit.acq commit))))
+(REL_UR : forall l' l : Loc.t,
+         max_value f (t_rel urr acts sb rmw rf sc (thread a) l' l)
+           (LocFun.find l (Capability.ur (LocFun.find l' (Commit.rel commit)))))
+(REL_UR0 : forall l' l : Loc.t,
+          max_value f (t_rel rwr acts sb rmw rf sc (thread a) l' l)
+            (LocFun.find l (Capability.rw (LocFun.find l' (Commit.rel commit)))))
+(REL_UR1 : forall l' l : Loc.t,
+          max_value f (t_rel scr acts sb rmw rf sc (thread a) l' l)
+            (LocFun.find l (Capability.sc (LocFun.find l' (Commit.rel commit)))))
+(STATE : Language.step lang (Some (ProgramEvent.read l v o)) st st')
+(RFb : rf0 b a)
+(INb : In b acts)
+(o_b : Ordering.t)
+(LABb : lab b = Astore l v o_b)
+(H : ~ is_fence a)
+(H0 : ~ is_write a)
+(E : Cell.get (f b) (Configuration.memory op_st l) =
+    Some (from, {| Message.val := v; Message.released := rel |}))
+(WRITE_B : is_write b)
+(LOC_B : loc b = Some l)
+(SIM_MEM0 : forall l : Loc.t, sim_cell f acts sb rmw rf sc (Configuration.memory op_st l) l)
+(HELPER : forall
+           (R : list event ->
+                relation event ->
+                relation event -> relation event -> relation event -> relation event)
+           (l0 : Loc.t) (x : event),
+         (fun x0 : event => msg_rel R acts sb rmw rf sc l0 x0 b) x <->
+         msg_rel R acts sb rmw rf sc l0 x b) :
+
+sim_commit f acts0 sb0 rmw0 rf0 sc0
+  (Commit.read_commit
+     (Local.commit {| Local.commit := commit; Local.promises := Memory.bot |}) l 
+     (f b) rel o) (thread a).
+Proof.
+
+assert (RLXa: is_rlx_rw a <-> Ordering.le Ordering.relaxed o).
+  unfold is_rlx_rw; rewrite LABa; done.
+assert (ACQa: is_acq a <-> Ordering.le Ordering.acqrel o).
+  unfold is_acq; rewrite LABa; done.
+assert (SCa: is_sc a <-> Ordering.le Ordering.seqcst o).
+  unfold is_sc; rewrite LABa; done.
+
+generalize (gstep_read_rf COH GSTEP LABa); intro; desc.
+
+
+
+generalize (gstep_t_rel_other GSTEP urr); intro REL_URR.
+assert (A: gstep_a a (urr acts sb rmw rf sc) (urr acts0 sb0 rmw0 rf0 sc0)).
+eapply gstep_urr_a; eauto.
+assert (B: inclusion (urr acts sb rmw rf sc) (urr acts0 sb0 rmw0 rf0 sc0)).
+eapply urr_mon; eauto.
+specialize (REL_URR A B (thread a)).
+clear A B.
+generalize (gstep_t_rel_other GSTEP rwr); intro REL_RWR.
+assert (A: gstep_a a (rwr acts sb rmw rf sc) (rwr acts0 sb0 rmw0 rf0 sc0)).
+eapply gstep_rwr_a; eauto.
+assert (B: inclusion (rwr acts sb rmw rf sc) (rwr acts0 sb0 rmw0 rf0 sc0)).
+eapply rwr_mon; eauto.
+specialize (REL_RWR A B (thread a)).
+clear A B.
+generalize (gstep_t_rel_other GSTEP scr); intro REL_SCR.
+assert (A: gstep_a a (scr acts sb rmw rf sc) (scr acts0 sb0 rmw0 rf0 sc0)).
+eapply gstep_scr_a; eauto.
+assert (B: inclusion (scr acts sb rmw rf sc) (scr acts0 sb0 rmw0 rf0 sc0)).
+eapply scr_mon; eauto.
+specialize (REL_SCR A B (thread a)).
+clear A B.
+
+destruct commit; simpl.
+
+unfold sim_commit, sim_acq, sim_cur, sim_rel; splits; ins.
+
+all: try rewrite LocFun.add_spec; desf.
+all: ins.
+all: try rewrite !tm_join_bot.
+all: try rewrite !tm_find_join.
+all: try rewrite !tm_find_singleton; desf.
+all: try rewrite !time_join_bot.
+all: do 2 (try match goal with
+| [|- max_value _ _ (Time.join _ _)] => eapply max_value_join  end).
+all: try match goal with
+       | [|- max_value _ _ (LocFun.find _ _)] => eapply max_value_same_set; eauto with acts
+       | [|- max_value _ _ _ ] => eapply max_value_singleton; eauto end.
+all: try by apply HELPER.
+all: simpl.
+all: try eapply helper.
+all: intro x.
+all: try (rewrite (gstep_t_cur_urr_read COH GSTEP b RFb); split; ins; desf; try by eauto; try by (exfalso; eauto)).
+all: try (rewrite (gstep_t_cur_rwr_read COH GSTEP b RFb); split; ins; desf; try by eauto; try by (exfalso; eauto)).
+all: try (rewrite (gstep_t_cur_scr_read COH GSTEP b RFb); split; ins; desf; try by eauto; try by (exfalso; eauto)).
+all: try (rewrite (gstep_t_acq_urr_read COH GSTEP b RFb); split; ins; desf; try by eauto; try by (exfalso; eauto)).
+all: try (rewrite (gstep_t_acq_rwr_read COH GSTEP b RFb); split; ins; desf; try by eauto; try by (exfalso; eauto)).
+all: try (rewrite (gstep_t_acq_scr_read COH GSTEP b RFb); split; ins; desf; try by eauto; try by (exfalso; eauto)).
+rewrite REL_URR; auto.
+rewrite REL_RWR; auto.
+rewrite REL_SCR; auto.
 Qed.
 
 (******************************************************************************)
@@ -617,8 +892,11 @@ eapply monotone_converse_strict with (acts:=(a :: acts)); eauto.
 - intro.
   eapply Coherent_scr; eauto.
   red in INa; red in INa; desc.
-  eapply S_tm_sc; eauto with acts.
+  eapply S_tm_sc with (b:=y); eauto with acts.
   eapply S_tmr_mon; eauto.
+apply SC_AT_END; eauto.
+apply S_tmr_domb in INa; done.
+- intro; subst; eauto with acts. 
 Qed.
 
 Lemma Writable_full acts sb rmw rf mo sc acts' sb' rmw' rf' mo' sc'
@@ -639,68 +917,100 @@ constructor; try intro.
 eapply Writable_cur_rwr; eauto.
 eapply Writable_cur_scr; eauto with acts.
 eapply Writable_sc_map; eauto with acts.
-Admitted.
+Qed.
 
 (******************************************************************************)
 (** * Main Theorem: the operational machine simulates the axiomatic machine   *)
 (******************************************************************************)
 
-Lemma foo (P Q : Prop) : P -> (P -> Q) -> P /\ Q.
-Proof. tauto. Qed.
 
-Lemma ax_op_sim_helper 
-op_st ax_st (SIM: sim op_st ax_st) ax_st' (AXSTEP: step ax_st ax_st')
-(NEXT: exists (e0 : option Event.t) (tid : Ident.t) threads sc_map memory,
-  Configuration.step e0 tid op_st 
-    {| Configuration.threads:=threads; Configuration.sc:=sc_map; 
-       Configuration.memory:=memory  |}
-  /\
-  sim {| Configuration.threads:=threads; Configuration.sc:=sc_map; 
-         Configuration.memory:=memory  |} ax_st') :
-  exists e tid op_st', Configuration.step e tid op_st op_st' /\ sim op_st' ax_st'.
-Proof.
-desf.
-eauto.
-Qed.
 
 Lemma ax_op_sim :
   forall op_st ax_st (SIM: sim op_st ax_st) ax_st' (AXSTEP: step ax_st ax_st'),
   exists e tid op_st', Configuration.step e tid op_st op_st' /\ sim op_st' ax_st'.
 Proof.
-ins.
+ins; red in SIM; desc.
 destruct AXSTEP.
-red in SIM; desc.
-red in SIM. desc. 
+
 rewrite STATES in TID.
 apply find_mapD in TID; desc; destruct z as [? local]; ins; desf.
+destruct local as [commit promises].
+assert (TID' := TID).
+apply NO_PROMISES in TID'; ins; subst.
 
-destruct MSTEP; subst.
-
-(** SILENT **)
+cut (exists te commit' sc' mem' op_st' threads' local', 
+<< OP_ST': op_st' = Configuration.mk threads' sc' mem' >> /\ 
+<< THREAD': threads' = IdentMap.add i 
+  (existT Language.state lang st', local') (Configuration.threads op_st) >> /\ 
+<< LOCAL': local' = Local.mk commit' Memory.bot >> /\ 
+<< STEP: Thread.program_step te 
+    (Thread.mk lang st (Local.mk commit Memory.bot) (Configuration.sc op_st) (Configuration.memory op_st))
+    (Thread.mk lang st' local' sc' mem') >> /\
+  << TIME: exists f', 
+    << F: forall b : event, In b (acts ax_st) -> f' b = f b >> /\
+    << MONOTONE: monotone (mo ax_st') f' >> /\  
+    << SIM_COMMIT: sim_commit f' (acts ax_st') (sb ax_st') (rmw ax_st') (rf ax_st') (sc ax_st') commit' i >> /\
+    << SIM_SC_MAP: forall l, max_value f' (S_tm (acts ax_st') (sb ax_st') (rmw ax_st') (rf ax_st') l) 
+        (LocFun.find l sc')  >> /\
+    << SIM_MEM: sim_mem f' (acts ax_st') (sb ax_st') (rmw ax_st') (rf ax_st') (sc ax_st') mem'  >> >>).
 {
-eexists _,i,_.
-split.
-econstructor; try edone.
-eauto.
-apply Thread.step_program.
-eapply Thread.step_silent; edone.
-admit.
-admit.
+  ins; desc.
+  eexists _,i,_.
+  apply foo; [|intro CSTEP].
+  -  econstructor; try edone; try apply Thread.step_program; eauto.
+    red; ins; eexists; splits; eauto; simpl; desf.
+  - red; simpl; splits; eauto.
+    * destruct MSTEP; eauto.
+      by rewrite <- SAME_ACTS, <- SAME_SB, <- SAME_RMW, <- SAME_RF, <- SAME_MO, <- SAME_SC.
+    * eapply Configuration.step_future; eauto.
+    * eapply Configuration.step_future; eauto.
+    * intro; rewrite IdentMap.gsspec. ins; desf; simpl; eapply NO_PROMISES; eauto.
+    * by rewrite IdentMap.map_add; simpl; rewrite MTS, STATES.
+    * eexists. splits; eauto; ins.
+      rewrite IdentMap.gsspec in TID0; desf; ins; simpl.
+      destruct MSTEP. 
+        rewrite <- SAME_ACTS, <- SAME_SB, <- SAME_RMW, <- SAME_RF, <- SAME_SC.
+        eapply sim_commit_other_threads_silent; eauto.
+      all: eapply sim_commit_other_threads; eauto 2.
+      all: try eapply sim_commit_other_threads; eauto 2.
+      all: intro; subst; eauto.
 }
 
-(** READ **)
+unnw. 
+apply SIM_COMMIT in TID.
+ins.
+clear NO_PROMISES SIM_COMMIT.
+destruct ax_st, ax_st'; simpl; ins.
+destruct MSTEP; ins; subst.
+
+
 {
-assert (SCa: is_sc a = Ordering.le Ordering.seqcst o).
-  unfold is_sc; unfold ord; rewrite LABa; done.
-assert (RAa: is_ra a = Ordering.le Ordering.acqrel o).
-  unfold is_ra; unfold ord; rewrite LABa; done.
-assert (RLXa: is_rlx a = Ordering.le Ordering.relaxed o).
-  unfold is_rlx; unfold ord; rewrite LABa; done.
+(** SILENT **)
+eexists _,_,_,_,_,_,_.
+splits; eauto.
+eapply Thread.step_silent; eauto.
+exists f; splits; eauto.
+}
+
+all: red in TID; desc; red in CUR; desc; red in ACQ; desc; red in REL; desc.
+
+{
+(** READ **)
+
+(* assert (RLXa: is_rlx_rw a <-> Ordering.le Ordering.relaxed o).
+  unfold is_rlx_rw; rewrite LABa; done.
+assert (ACQa: is_acq a <-> Ordering.le Ordering.acqrel o).
+  unfold is_acq; rewrite LABa; done.
+assert (SCa: is_sc a <-> Ordering.le Ordering.seqcst o).
+  unfold is_sc; rewrite LABa; done. *)
 
 generalize (gstep_read_rf COH GSTEP LABa); intro; desc.
 
-assert (~ is_wfence a /\ ~ is_write a).
-  unfold is_write, is_wfence; destruct (lab a); ins.
+
+
+
+assert (~ is_fence a /\ ~ is_write a).
+  unfold is_write, is_fence; destruct (lab a); ins.
 
 assert (E: exists from rel, Cell.get (f b) ((Configuration.memory op_st) l) = 
           Some (from, {| Message.val:=v; Message.released:=rel |})).
@@ -713,144 +1023,330 @@ assert (WRITE_B: is_write b).
 assert (LOC_B: Gevents.loc b = Some l). 
   unfold Gevents.loc; destruct (lab b); ins; desf.
 
-cdes MEM. specialize (MEM l); red in MEM; desc.
+cdes SIM_MEM. specialize (SIM_MEM l); red in SIM_MEM; desc.
 specialize (SIMCELL b WRITE_B LOC_B from 
   {| Message.val := v; Message.released := rel |} E).
 red in SIMCELL; desc; red in SIMMSG; desc.
 
-eexists _,(thread a),_.
-apply foo; [|intro STEP].
-{
-econstructor; try edone.
-eauto.
-apply Thread.step_program; try edone.
-  eapply Thread.step_read; eauto.
-  econstructor; try edone.
-  specialize (LOCAL (thread a) (existT _ lang st) local TID); desf.
-  red in LOCAL; red in LOCAL; desc; red in CUR; desc.
-  eapply Readable_full; eauto.
-admit.
-}
-red; simpl; splits; eauto.
-- eby eapply Configuration.step_future.
-- eby eapply Configuration.step_future.
-- ins; rewrite IdentMap.gsspec in TID0; desf; ins;
-  eapply NO_PROMISES; edone.
-- rewrite IdentMap.map_add. admit.
-- clear STEP.
-
-exists f; split.
+eexists _,_,_,_,_,_,_.
+splits; eauto.
+eapply Thread.step_read; eauto.
+econstructor; eauto.
+eapply Readable_full; eauto.
+exists f; splits; eauto.
 * rewrite <- gstep_non_write_mo; eauto with acts.
-* red; splits; ins.
-  + ins; rewrite IdentMap.gsspec in TID0; desf; ins.
-    Focus 2. by eapply sim_local_other_threads; eauto.
-    red; ins; red; ins.
-    exploit LOCAL; clear LOCAL; eauto; intro LOCAL; unfold sim_local in *; ins.
-    unfold sim_commit, sim_acq, sim_cur, sim_rel in *; desc; splits; intro l';
-    simpl;
-    unfold TimeMap.bot.
-    all: try (rewrite !tm_join; rewrite time_join_bot).
-    all: try (rewrite !tm_join; rewrite tm_join_singleton_to_if).
-    all: try rewrite !time_join_bot.
-    all: try rewrite !fun_if; simpl.
-    all: try rewrite !if_arg with (x := l'); simpl.
-    all: unfold TimeMap.bot; simpl.
-    all: try intro; try eapply max_value_join_if_loc; try edone; simpl.
-    all: try intro; try eapply max_value_join_if; try edone.
-    all: try intro; try eapply max_value_same_set; try edone.
-    all: try rewrite <- RAa; try rewrite <- RLXa; try rewrite <- SCa.
-
-
-
-    eapply gstep_t_cur_urr_read; eauto.
-    eapply gstep_t_cur_rwr_read; eauto.
-    eapply gstep_t_cur_scr_read; eauto.
-    eapply gstep_t_acq_urr_read; eauto.
-    admit.
-    admit.
-    intro; symmetry; eapply gstep_t_rel_other; eauto using gstep_urr_a, urr_mon.
-    intro; symmetry; eapply gstep_t_rel_other; eauto using gstep_rwr_a, rwr_mon.
-    intro; symmetry; eapply gstep_t_rel_other; eauto using gstep_scr_a, scr_mon.
-+ eapply max_value_same_set; try edone.
-admit.
-+ admit.
+* eapply commit_step_read; eauto.
+* ins. eapply max_value_same_set; try edone.
+ins; rewrite gstep_S_tm_other; eauto with acts.
+* red; ins.
+  specialize (SIM_MEM0 l0); red in SIM_MEM0; desf.
+  red; splits; eauto; ins.
+  specialize (SIMCELL b0 WRITE LOC from0 msg CELL).
+  unfold sim_cell_helper, sim_msg in *; desc; splits; eauto.
+  4: by ins; apply FROMRMW0; eapply gstep_rf_rmw with (rf' := rf0); eauto.
+  all: ins.
+  all: destruct msg; ins.
+  all:  eapply max_value_same_set; try edone.
+  all: simpl.
+  admit.
+  admit.
+  admit. 
 }
-
-
-(** Write **)
 {
+(** Write **)
+
 generalize (new_f GSTEP MONOTONE); intro; desc.
 
 assert (LOC_A: Gevents.loc a = Some l). 
   unfold Gevents.loc; destruct (lab a); ins; desf.
 
 
-eexists _,(thread a),_.
-apply foo; [|intro STEP].
-{
-econstructor; try edone.
-eauto.
-apply Thread.step_program; try edone.
-eapply Thread.step_write with (to:= f' a); eauto.
-econstructor; try edone.
-specialize (LOCAL (thread a) (existT _ lang st) local TID); desf.
-red in LOCAL; red in LOCAL; desc; red in CUR; desc.
+eexists _,_,_,_,_,_,_. splits; eauto.
+eapply Thread.step_write; eauto.
+econstructor; eauto.
 eapply Writable_full; eauto.
+
+{
 admit.
+
+}
+
+assert (WRITE: is_write a).
+  eauto with acts.
+assert (NR: ~ is_read a).
+  eauto with acts.
+
+assert (SCa: Ordering.le Ordering.seqcst o <-> is_sc a).
+  split; eauto with acts. unfold is_sc; destruct (lab a); ins; desf.
+assert (RAa: Ordering.le Ordering.acqrel o <-> is_rel a).
+  split; eauto with acts. unfold is_rel; destruct (lab a); ins; desf.
+
+
+
+
+destruct op_st; ins.
+
+exists f'; splits; try done.
+{
+destruct commit; simpl.
+unfold Commit.write_commit.
+
+all: unfold sim_commit; splits; ins.
+- generalize (gstep_t_cur_urr_write COH GSTEP WRITE); intro CUR_URR.
+  generalize (gstep_t_cur_rwr_write COH GSTEP WRITE); intro CUR_RWR.
+  generalize (gstep_t_cur_scr_write COH GSTEP WRITE); intro CUR_SCR.
+  destruct cur as [cur_ur cur_rw cur_sc]; unfold sim_cur; splits; ins.
+  all: try rewrite !tm_find_join.
+  all: try rewrite !tm_find_singleton; desf; ins.
+  all: try rewrite !time_join_bot.
+  all: try eapply max_value_join; try eapply max_value_join.
+  all: try match goal with
+         | [|- max_value _ _ (LocFun.find _ _)] => eapply max_value_same_set;
+           try eapply max_value_new_f with (f':=f'); eauto with acts
+         | [|- max_value _ _ _ ] => eapply max_value_singleton; eauto
+       end.
+  all: try by intro x; split; [intro K; pattern x; exact K|].
+  all: ins.
+  all: try rewrite CUR_URR.
+  all: try rewrite CUR_RWR.
+  all: try rewrite CUR_SCR.
+  all: split; ins; desf; try by eauto.
+  all: by exfalso; eauto.
+
+- 
+
+  assert (ACQ_URR : forall (l : Loc.t) (x : event),
+          t_acq urr acts0 sb0 rmw0 rf0 sc0 (thread a) l x <->
+          t_acq urr acts sb rmw rf sc (thread a) l x \/
+          x = a /\ loc x = Some l).
 admit.
+assert (ACQ_RWR : forall (l : Loc.t) (x : event),
+          t_acq rwr acts0 sb0 rmw0 rf0 sc0 (thread a) l x <->
+          t_acq rwr acts sb rmw rf sc (thread a) l x \/
+          x = a /\ loc x = Some l).
+admit.
+assert (ACQ_SCR : forall (l : Loc.t) (x : event),
+          t_acq scr acts0 sb0 rmw0 rf0 sc0 (thread a) l x <->
+          t_acq scr acts sb rmw rf sc (thread a) l x \/
+          S_tm acts sb rmw rf l x /\ is_sc a \/ x = a /\ loc x = Some l).
+admit.
+destruct acq as [acq_ur acq_rw acq_sc]; unfold sim_acq; splits; ins.
+
+  all: try rewrite !tm_find_join.
+  all: try rewrite !tm_find_singleton; desf; ins.
+  all: try rewrite !time_join_bot.
+  all: try eapply max_value_join; try eapply max_value_join.
+  all: try match goal with
+         | [|- max_value _ _ (LocFun.find _ _)] => eapply max_value_same_set;
+           try eapply max_value_new_f with (f':=f'); eauto with acts
+         | [|- max_value _ _ _ ] => eapply max_value_singleton; eauto
+       end.
+  all: try by intro x; split; [intro K; pattern x; exact K|].
+
+  all: ins.
+  all: try rewrite ACQ_URR.
+  all: try rewrite ACQ_RWR.
+  all: try rewrite ACQ_SCR.
+  all: split; ins; desf; try by eauto.
+  all: try by exfalso; eauto.
+
+- generalize (gstep_t_rel_urr_write COH GSTEP WRITE LOC_A); intro REL_URR.
+  generalize (gstep_t_rel_rwr_write COH GSTEP WRITE LOC_A); intro REL_RWR.
+  generalize (gstep_t_rel_scr_write COH GSTEP WRITE LOC_A); intro REL_SCR.
+(*  assert (REL_URR': forall (l0 l' : Loc.t), ~ is_rel a \/ Some l <> Some l0 -> 
+            forall x, t_rel urr acts0 sb0 rmw0 rf0 sc0 (thread a) l0 l' x <->
+                      t_rel urr acts sb rmw rf sc (thread a) l0 l' x).
+    ins; rewrite gstep_t_rel_other; eauto.
+    eapply gstep_urr_a; eauto.
+    eapply urr_mon; eauto.
+    desf; eauto.
+    right; right; right; splits; eauto.
+    ins; intro; subst; destruct (loc a); ins; desf; auto.
+ *)
+
+assert (FOO: forall r l l' x,
+  t_rel r acts sb rmw rf sc (thread a) l l' x ->
+  t_cur r acts sb rmw rf sc (thread a) l' x).
+admit.
+
+unfold sim_rel; splits; ins.
+
+all: try rewrite LocFun.add_spec; desf; ins.
+  all: try rewrite !tm_join_bot.
+
+  all: try rewrite !tm_find_join.
+  all: try rewrite !tm_find_singleton; desf; ins.
+  all: try rewrite !time_join_bot.
+
+  all: try eapply max_value_join; try eapply max_value_join.
+  all: try match goal with
+         | [|- max_value _ _ (LocFun.find _ _)] => eapply max_value_same_set;
+           try eapply max_value_new_f with (f':=f'); eauto with acts
+         | [|- max_value _ _ _ ] => eapply max_value_singleton; eauto
+       end.
+  all: try by intro x; split; [intro K; pattern x; exact K|].
+
+  all: ins.
+  all: try rewrite REL_URR.
+  all: try rewrite REL_RWR.
+  all: try rewrite REL_SCR.
+  all: try rewrite (gstep_t_rel_other GSTEP _ (gstep_urr_a COH GSTEP) (urr_mon GSTEP)).
+  all: try rewrite (gstep_t_rel_other GSTEP _ (gstep_rwr_a COH GSTEP) (rwr_mon GSTEP)).
+  all: try rewrite (gstep_t_rel_other GSTEP _ (gstep_scr_a COH GSTEP) (scr_mon GSTEP)).
+  all: try (repeat right; split; ins; congruence).
+  all: try (split; ins; desf; eauto).
+  all: eauto 8.
+  all: try by exfalso; eauto.
+
+  by exploit RAa0; try done; destruct a as [??[]]; ins; destruct o0; ins.
+}
+{
+ins.
+unfold Commit.write_sc; desf; ins.
+all: try rewrite !tm_find_join.
+all:  try   rewrite !tm_find_singleton; desf; ins.
+all:  try   rewrite time_join_bot.
+all: try eapply max_value_join.
+all: try match goal with
+         | [|- max_value _ _ (LocFun.find _ _)] => eapply max_value_same_set;
+           try eapply max_value_new_f with (f':=f'); eauto with acts
+         | [|- max_value _ _ _ ] => eapply max_value_singleton; eauto
+       end.
+all: ins.
+all: rewrite gstep_S_tm_write; eauto.
+all: split; ins; desf; eauto.
+all: try by (exfalso; eauto).
+}
+{
+admit.
+}
+}
+{
+(** Update **)
+admit.
+}
+{
+(** Fence **)
+
+assert (FENCE: is_fence a).
+  by destruct a; ins; desf.
+assert (NR: ~ is_read a).
+  eauto with acts.
+
+assert (SCa: Ordering.le Ordering.seqcst o_w <-> is_sc a).
+  by destruct a; ins; desf.
+assert (RAa: Ordering.le Ordering.acqrel o_r <-> is_acq a).
+  by destruct a; ins; desf.
+assert (RAr: Ordering.le Ordering.acqrel o_w <-> is_rel a).
+  by destruct a; ins; desf.
+
+
+destruct op_st as [threads sc_map mem]; ins.
+
+eexists _,_,_,_,_,_,_.
+splits; eauto.
+eapply Thread.step_fence; eauto.
+econstructor; eauto.
+exists f; splits; eauto.
+
+* rewrite <- gstep_non_write_mo; eauto with acts.
+  intro; unfold is_write in *; destruct (lab a); ins.
+* simpl.
+
+assert (forall acts sb rmw rf sc, inclusion (urr acts sb rmw rf sc) (rwr acts sb rmw rf sc)).
+by vauto.
+assert (forall acts sb rmw rf sc, inclusion (rwr acts sb rmw rf sc) (scr acts sb rmw rf sc))
+by vauto.
+
+assert (FOOca: forall r r' l x,
+  t_cur r acts sb rmw rf sc (thread a) l x ->
+  (forall acts sb rmw rf sc, inclusion (r acts sb rmw rf sc) (r' acts sb rmw rf sc)) ->
+  t_acq r' acts sb rmw rf sc (thread a) l x).
+admit.
+
+assert (FOOaa: forall r r' l x,
+  t_acq r acts sb rmw rf sc (thread a) l x ->
+  (forall acts sb rmw rf sc, inclusion (r acts sb rmw rf sc) (r' acts sb rmw rf sc)) ->
+  t_acq r' acts sb rmw rf sc (thread a) l x).
+admit.
+
+assert (FOOcc: forall r r' l x,
+  t_cur r acts sb rmw rf sc (thread a) l x ->
+  (forall acts sb rmw rf sc, inclusion (r acts sb rmw rf sc) (r' acts sb rmw rf sc)) ->
+  t_cur r' acts sb rmw rf sc (thread a) l x).
+admit.
+
+assert (FOOrc: forall r l l' x,
+  t_rel r acts sb rmw rf sc (thread a) l l' x ->
+  t_cur r acts sb rmw rf sc (thread a) l' x).
+admit.
+
+assert (FOOra: forall r l l' x,
+  t_rel r acts sb rmw rf sc (thread a) l l' x ->
+  t_acq r acts sb rmw rf sc (thread a) l' x).
+admit.
+
+
+destruct commit; ins.
+unfold Commit.write_fence_commit, Commit.read_fence_commit,
+       Commit.write_fence_sc; ins; desf.
+all: try rewrite !cap_join_bot.
+all: unfold sim_commit, sim_acq, sim_cur, sim_rel; splits; ins.
+
+all: desf.
+all: try rewrite !tm_join_bot.
+all: try rewrite !tm_find_join.
+all: try rewrite !tm_find_singleton; desf.
+all: try rewrite !time_join_bot.
+all: do 2 (try match goal with
+| [|- max_value _ _ (Time.join _ _)] => eapply max_value_join  end).
+all: try match goal with
+       | [|- max_value _ _ (LocFun.find _ _)] => eapply max_value_same_set; eauto with acts
+       | [|- max_value _ _ _ ] => eapply max_value_singleton; eauto end.
+  all: try by intro x; split; [intro K; pattern x; exact K|].
+all: simpl.
+all: intro x.
+
+all: try rewrite (gstep_t_acq_urr_nonread COH GSTEP NR).
+all: try rewrite (gstep_t_acq_rwr_nonread COH GSTEP NR).
+all: try rewrite (gstep_t_acq_scr_nonread COH GSTEP NR).
+
+all: try rewrite (gstep_t_cur_urr_fence COH GSTEP FENCE).
+all: try rewrite (gstep_t_cur_rwr_fence COH GSTEP FENCE).
+all: try rewrite (gstep_t_cur_scr_fence COH GSTEP FENCE).
+
+all: try rewrite (gstep_t_rel_urr_fence COH GSTEP FENCE).
+all: try rewrite (gstep_t_rel_rwr_fence COH GSTEP FENCE).
+all: try rewrite (gstep_t_rel_scr_fence COH GSTEP FENCE).
+
+
+  all: try (split; ins; desf; eauto).
+  all: try by exfalso; eauto.
+  all: try by destruct o_w.
+  all: eauto using inclusion_refl2.
+  all: eauto 8 using inclusion_refl2, ur_in_sc, ur_in_rw, rw_in_sc.
+all: admit.
+
+* ins. eapply max_value_same_set; try edone.
+ins; rewrite gstep_S_tm_other; eauto with acts.
+* red; ins.
+  specialize (SIM_MEM0 l0); red in SIM_MEM0; desf.
+  red; splits; eauto; ins.
+  specialize (SIMCELL b0 WRITE LOC from0 msg CELL).
+  unfold sim_cell_helper, sim_msg in *; desc; splits; eauto.
+  4: by ins; apply FROMRMW0; eapply gstep_rf_rmw with (rf' := rf0); eauto.
+  all: ins.
+  all: destruct msg; ins.
+  all:  eapply max_value_same_set; try edone.
+  all: simpl.
+  admit.
+  admit.
+  admit. 
+}
+
 admit.
 }
 
-red; simpl; splits; eauto.
-- eby eapply Configuration.step_future.
-- eby eapply Configuration.step_future.
-- ins; rewrite IdentMap.gsspec in TID0; desf; ins;
-  eapply NO_PROMISES; edone.
-- rewrite IdentMap.map_add. admit.
--
-  exists f'; splits; try done.
-   red; splits; ins.
-  + ins; rewrite IdentMap.gsspec in TID0; desf; ins.
-    Focus 2.  eapply sim_local_other_threads'; eauto.
-    red; ins; red; ins.
-    exploit LOCAL; clear LOCAL; eauto; intro LOCAL; unfold sim_local in *; ins.
-    unfold sim_commit, sim_acq, sim_cur, sim_rel in *; desc; splits; intro l';
-    simpl.
-    all: unfold TimeMap.bot, LocFun.add; simpl.
-    all: try (rewrite !tm_join; rewrite time_join_bot).
-    all: try (rewrite !tm_join; rewrite tm_join_singleton_to_if).
-    all: try rewrite !time_join_bot.
-    all: try rewrite !fun_if; simpl.
-    all: try rewrite !if_arg with (x := l'); simpl.
-    all: unfold TimeMap.bot; simpl.
-all: try rewrite !if_same.
-    all: try rewrite !time_join_bot.
-
-
-all: try eapply max_value_join_loc; eauto with acts; simpl.
-
-    all: try intro; try eapply max_value_join_if_loc; eauto with acts; simpl.
-    all: try intro; try eapply max_value_join_if; eauto with acts; simpl.
-
-
-    all: try intro; try eapply max_value_same_set; try edone.
-    all: try rewrite <- RAa; try rewrite <- RLXa; try rewrite <- SCa.
-    eapply gstep_t_cur_urr_write; eauto.
-    eapply gstep_t_cur_rwr_read; eauto.
-    eapply gstep_t_cur_scr_read; eauto.
-    eapply gstep_t_acq_urr_read; eauto.
-    admit.
-    admit.
-    intro; symmetry; eapply gstep_t_rel_other; eauto using gstep_urr_a, urr_mon.
-    intro; symmetry; eapply gstep_t_rel_other; eauto using gstep_rwr_a, rwr_mon.
-    intro; symmetry; eapply gstep_t_rel_other; eauto using gstep_scr_a, scr_mon.
-+ eapply max_value_same_set; try edone.
-admit.
-+ admit.
-
-
-
-}
 Admitted.
 
 Lemma ax_sim_op :
