src/axiomatic/Machine.v
@@ -37,16 +37,14 @@ Record configuration :=
     mo : event -> event -> Prop ; 
     sc : event -> event -> Prop }.
 
-Definition id_gstep mc mc' : Prop :=
-  << SAME_ACTS: acts mc = acts mc' >> /\
-  << SAME_SB: sb mc = sb mc' >> /\
-  << SAME_RMW: rmw mc = rmw mc' >> /\
-  << SAME_RF: rf mc = rf mc' >> /\
-  << SAME_MO: mo mc = mo mc' >> /\
-  << SAME_SC: sc mc = sc mc' >>.
-
 Inductive mstep mc mc' e i : Prop :=
-  | silent (SILENT: e = None) (ID_GRAPH: id_gstep mc mc')
+  | silent (SILENT: e = None) 
+      (SAME_ACTS: acts mc = acts mc')
+      (SAME_SB: sb mc = sb mc') 
+      (SAME_RMW: rmw mc = rmw mc') 
+      (SAME_RF: rf mc = rf mc')
+      (SAME_MO: mo mc = mo mc') 
+      (SAME_SC: sc mc = sc mc')
   | read a l v o 
       (EVENT: e = Some (ProgramEvent.read l v o)) 
       (LABa: lab a = Aload l v o) 
@@ -68,14 +66,11 @@ Inductive mstep mc mc' e i : Prop :=
            (acts mc_mid) (sb mc_mid) (rmw mc_mid) (rf mc_mid) (mo mc_mid) (sc mc_mid) a_r)
       (GSTEPw: gstep (acts mc_mid) (sb mc_mid) (rmw mc_mid) (rf mc_mid) (mo mc_mid) (sc mc_mid)
                      (acts mc') (sb mc') (rmw mc') (rf mc') (mo mc') (sc mc') a_w)
-  | fence a_r a_w o_r o_w (EVENT: e = Some (ProgramEvent.fence o_r o_w)) 
-      (LABar: lab a_r = Arfence o_r) (LABaw: lab a_w = Awfence o_w) 
-      (TIDar: thread a_r = i) (TIDaw: thread a_w = i) 
-      mc_mid
-      (GSTEPr: gstep (acts mc) (sb mc) (rmw mc) (rf mc) (mo mc) (sc mc)
-           (acts mc_mid) (sb mc_mid) (rmw mc_mid) (rf mc_mid) (mo mc_mid) (sc mc_mid) a_r)
-      (GSTEPw: gstep (acts mc_mid) (sb mc_mid) (rmw mc_mid) (rf mc_mid) (mo mc_mid) (sc mc_mid)
-                     (acts mc') (sb mc') (rmw mc') (rf mc') (mo mc') (sc mc') a_w).
+  | fence a o_r o_w (EVENT: e = Some (ProgramEvent.fence o_r o_w)) 
+      (LABa: lab a = Afence o_r o_w) 
+      (TIDa: thread a = i) 
+      (GSTEP: gstep (acts mc) (sb mc) (rmw mc) (rf mc) (mo mc) (sc mc)
+                    (acts mc') (sb mc') (rmw mc') (rf mc') (mo mc') (sc mc') a).
 
 Inductive step mc mc' : Prop :=
 | step_intro  
